hey

Translation.v
@@ -13,8 +13,8 @@ Set Implicit Arguments.
 
 Open Scope pred.
 
-Definition sep_base (x:var) (t:base_type) : pred world :=
-  EX v : (base_of_type t), (fun s => (eval s (var_e x) = (val_of_base t v))).
+Definition sep_base (x:expr) (t:base_type) : pred world :=
+  EX v : (base_of_type t), (fun s => (eval s x = (val_of_base t v))).
 
 Fixpoint sep_pred (p:reft_prop) : pred world :=
   match p with
@@ -28,23 +28,23 @@ Fixpoint sep_pred (p:reft_prop) : pred world :=
     | or_r p1 p2 => sep_pred p1 || sep_pred p2
   end.
 
-Definition sep_ty (x:var) (t:reft_type) : pred world :=
+Definition sep_ty (x:expr) (t:reft_type) : pred world :=
   match t with
-  | mkReft_type b p => sep_base x b && (sep_pred (subst (subst_one ν (var_e x)) p))
+  | mkReft_type b p => sep_base x b && (sep_pred (subst (subst_one ν x) p))
   end.
 
-Definition sep_base_e (e:expr) (t:base_type) : pred world :=
-  EX v : (base_of_type t), (fun s => (eval s e = (val_of_base t v))).
+(* Definition sep_base_e (e:expr) (t:base_type) : pred world := *)
+(*   EX v : (base_of_type t), (fun s => (eval s e = (val_of_base t v))). *)
 
-Definition sep_ty_e (e:expr) (t:reft_type) : pred world :=
-  match t with
-  | mkReft_type b p => sep_base_e e b && (sep_pred (subst (subst_one ν e) p))
-  end.
+(* Definition sep_ty_e (e:expr) (t:reft_type) : pred world := *)
+(*   match t with *)
+(*   | mkReft_type b p => sep_base_e e b && (sep_pred (subst (subst_one ν e) p)) *)
+(*   end. *)
 
 Fixpoint sep_env (Γ : type_env) : pred world :=
   match Γ with
     | nil => TT
-    | (x,t) :: Γ' => sep_ty x t && sep_env Γ'
+    | (x,t) :: Γ' => sep_ty (var_e x) t && sep_env Γ'
   end.
 
 Fixpoint sep_guards (Δ : guards) : pred world :=
@@ -56,7 +56,7 @@ Fixpoint sep_guards (Δ : guards) : pred world :=
 Definition sep_schema (f:pname) (s:stmt) (S:proc_schema) : procspec := 
   match S with
     | mkSchema xs ts (x, t) =>
-      (f, mkProc xs x [] s, sep_env (combine xs ts), sep_ty x t)
+      (f, mkProc xs x [] s, sep_env (combine xs ts), sep_ty (var_e x) t)
   end.
 
 Fixpoint sep_proc_env (Φ : proc_env) : procspecs :=
